ADD: `of_val`, `to_val`, `subst`

theories/ast.v
@@ -16,40 +16,37 @@ Inductive binop :=
 | PlusOp        (* +  *)
 | MinusOp       (* -  *)
 | MultOp        (* *  *)
-| DivOp         (* /  *)
+| QuotOp        (* /  *)
+| RemOp         (* %  *)
 | LtOp          (* <  *)
-| LteOp         (* <= *)
+| LeOp          (* <= *)
 | GtOp          (* >  *)
-| GteOp         (* >= *)
+| GeOp          (* >= *)
 | EqOp          (* == *)
 | NotEqOp       (* != *)
 | AndOp         (* && *)
 | OrOp          (* || *)
-| ShiftLeftOp   (* << *)
+| ShiftLOp      (* << *)
+| ShiftROp      (* >> *)
 | EndLeftOp     (* <| *)
 | DotOp         (* .  *)
 .
 
 (* leave out This, None, Ref, Some, Ok, and Err expressions *)
 Inductive sl_expr :=
-| Skip
-| NExpr (n: nat) (* assume in range of bits *)
-| ZExpr (n: Z)   (* assume in range of bits *)
-| StringExpr (val: string)
+| ValExpr (v: sl_val)
 | VarExpr (name: string)
 | ListExpr (exprs: list sl_expr)
 | BinaryExpr (op: binop) (lhs rhs: sl_expr)
 | TernaryExpr (cond if_true if_false: sl_expr)
-| CallExpr (name: string) (args: list sl_expr)
+| CallExpr (func: sl_expr) (args: list sl_expr)
 (* assume that type inferrence is not used and type is always provided *)
 | DeclareExpr (name: string) (mutable: bool) (type: sl_type) (expr: sl_expr)
 | AssignExpr (name: string) (expr: sl_expr)
 | ClosureExpr (args: list string) (body: sl_expr)
 | WhileExpr (cond body: sl_expr)
-| SeqExpr (e1 e2: sl_expr)
-.
-
-Inductive sl_val :=
+| Seq (exprs: list sl_expr)
+with sl_val :=
 | NVal (n: nat)
 | ZVal (n: Z)
 | StringVal (val: string)
@@ -57,42 +54,38 @@ Inductive sl_val :=
 | ClosureVal (args: list string) (body: sl_expr)
 .
 
-Fixpoint of_val (v: sl_val): sl_expr :=
-    match v with
-    | NVal n => NExpr n
-    | ZVal n => ZExpr n
-    | StringVal val => StringExpr val
-    | ListVal vals => ListExpr (List.map of_val vals)
-    | ClosureVal args body => ClosureExpr args body
-    end.
+Notation of_val := ValExpr (only parsing).
 
-Fixpoint to_val (e: sl_expr): option sl_val :=
+Definition to_val (e: sl_expr): option sl_val :=
     match e with
-    | NExpr n => Some (NVal n)
-    | ZExpr n => Some (ZVal n)
-    | StringExpr val => Some (StringVal val)
-    | ListExpr exprs =>
-        let fix test (tail: list sl_expr): option (list sl_val) :=
-            match tail with
-            | nil => Some nil
-            | cons x xs => match to_val x with
-                | None => None
-                | Some val => match test xs with
-                    | None => None
-                    | Some vals => Some (cons val vals)
-        end end end in
-        match test exprs with
-        | None => None
-        | Some vals => Some (ListVal vals)
-        end
-    | ClosureExpr args body => Some (ClosureVal args body)
+    | of_val v => Some v
     | _ => None
     end.
 
-Definition is_val (e: sl_expr): Prop :=
-    match to_val e with
-    | Some _ => True
-    | None => False
+Lemma to_of_val v: to_val (of_val v) = Some v.
+Proof.
+    destruct v; try reflexivity.
+Qed.
+
+Lemma of_to_val e v: to_val e = Some v -> of_val v = e.
+Proof.
+    destruct e; intro H; try discriminate.
+    f_equal. injection H as H. symmetry. assumption.
+Qed.
+
+Fixpoint subst (x: string) (v: sl_val) (e: sl_expr): sl_expr :=
+    match e with
+    | ValExpr _ => e
+    | VarExpr name => if String.eqb name x then of_val v else VarExpr name
+    | ListExpr exprs => ListExpr (List.map (subst x v) exprs)
+    | BinaryExpr op lhs rhs => BinaryExpr op (subst x v lhs) (subst x v rhs)
+    | TernaryExpr cond if_true if_false => TernaryExpr (subst x v cond) (subst x v if_true) (subst x v if_false)
+    | CallExpr func args => CallExpr (subst x v func) (List.map (subst x v) args)
+    | DeclareExpr name mutable type expr => DeclareExpr name mutable type (subst x v expr)
+    | AssignExpr name expr => AssignExpr name (subst x v expr)
+    | ClosureExpr args body => if List.existsb (String.eqb x) args then e else ClosureExpr args (subst x v body)
+    | WhileExpr cond body => WhileExpr (subst x v cond) (subst x v body)
+    | Seq exprs => Seq (List.map (subst x v) exprs)
     end.
 
 Record sl_function := {
@@ -105,4 +98,4 @@ Record sl_function := {
 
 Definition program := prod (list sl_function) sl_expr.
 
-Definition empty_program : program := (nil, Skip).
+Definition empty_program: program := (nil, Skip).
